Pearls/CelebrityCliques.dfy
@@ -1,0 +1,178 @@
+include "../examples/combinatorics.dfy"
+include "../lib/seq.dfy"
+include "./SeqFunctions.dfy"
+
+module CelebrityCliques {
+    import opened Combinatorics
+    import opened SeqCustom
+    import opened SeqFunctions
+    // import opened Std.Collections.Seq
+
+
+
+    predicate Knows<Person>(a: Person, b: Person)
+
+    predicate IsCelebrityClique<Person>(cs: set<Person>, ps: set<Person>)
+    {
+        cs <= ps && forall x :: x in ps ==> (forall y :: y in cs ==> Knows(x, y) && (Knows(y, x) ==> x in cs))
+    }
+
+    lemma CelebrityCliqueIsUnique<Person>(ps: set<Person>, cs: set<Person>, cs': set<Person>)
+        requires IsCelebrityClique(cs, ps)
+        requires IsCelebrityClique(cs', ps)
+        requires cs != {} && cs' != {}
+        requires cs != cs'
+        ensures false
+    {
+        // var c1 :| c1 in cs;
+        // var c2 :| c2 in cs';
+        // assert cs == cs' by {
+        //     forall c1 | c1 in cs
+        //         ensures c1 in cs'
+        //     {
+        //         var c2 :| c2 in cs';
+        //         // assert c2 in ps;
+        //         // assert c1 in ps;
+        //         // assert Knows(c1, c2);
+        //         // assert Knows(c2, c1);
+        //         // assert c1 in cs';
+        //     }
+
+        //     forall c2 | c2 in cs'
+        //         ensures c2 in cs
+        //     {
+        //         var c1 :| c1 in cs;
+        //         // assert c2 in ps;
+        //         // assert c1 in ps;
+        //     }
+        // }
+    }
+
+    function prepend<T(==)>(x: T, xs: seq<T>): seq<T> {
+        [x]+ xs
+    }
+
+    function subsetSeqs<T(==)>(xs: seq<T>): seq<seq<T>>
+        requires distinct(xs)
+    {
+        if xs == [] then
+            [[]]
+        else
+            Map((ss: seq<T>) => prepend(xs[0], ss), subsetSeqs(xs[1..]))
+            +
+            subsetSeqs(xs[1..])
+    }
+
+    function seqSeqsToSet<T(==)>(xs: seq<T>): set<set<T>>
+        requires distinct(xs)
+    {
+        set yy | yy in subsetSeqs(xs) :: ToSet(yy)
+    }
+
+    lemma subsetSeqsPowerset<T(==)>(xs: seq<T>)
+        requires distinct(xs)
+        ensures forall ss :: ss in PowerSet(ToSet(xs)) ==> ss in seqSeqsToSet(xs)
+    {
+        if xs == [] {
+            assert ToSet(xs) == {};
+            PowerSetEmptySet<T>({});
+            assert PowerSet(ToSet(xs)) == {{}};
+
+            assert forall ss :: ss in PowerSet(ToSet(xs)) ==> ss in seqSeqsToSet(xs);
+        } else if |xs| == 1 {
+            var x := xs[0];
+            assert ToSet(xs) == {xs[0]};
+            assert |Map((ss: seq<T>) => [xs[0]]+ss, [[]])| == 1;
+            var f := (ss: seq<T>) => prepend(xs[0], ss);
+            assert Map(f, [[]])[0] == f([]);
+            assert f([]) == [x];
+            calc {
+                subsetSeqs(xs);
+                Map(f, subsetSeqs(xs[1..]))+subsetSeqs(xs[1..]);
+                Map(f, subsetSeqs(xs[1..]))+[[]];
+                Map(f, [[]])+[[]];
+                [[xs[0]]]+[[]];
+                [[x],[]];
+            }
+            assert ToSet([x]) == {x};
+            assert {} in seqSeqsToSet(xs);
+            assert {x} in seqSeqsToSet(xs);
+            PowerSetOneElem(ToSet(xs), x);
+            assert PowerSet(ToSet(xs)) == {{},{x}};
+            // assert [x] in subsetSeq(xs);
+            assert forall ss :: ss in PowerSet(ToSet(xs)) ==> ss in seqSeqsToSet(xs);
+        }else {
+            subsetSeqsPowerset(xs[1..]);
+            var x := xs[0];
+            var f := (ss: seq<T>) => prepend(xs[0], ss);
+            calc {
+                subsetSeqs(xs);
+                Map(f, subsetSeqs(xs[1..]))+subsetSeqs(xs[1..]);
+            }
+            assert xs == [x] + xs[1..];
+            // var withX := set ss | ss in PowerSet(ToSet(xs[1..])) :: ss+{x};
+            var mapped := Map(f, subsetSeqs(xs[1..]));
+            // assert forall xx :: xx in mapped ==> ToSet(xx) in PowerSet(ToSet(xs));
+            // assert forall wx :: wx in withX ==> wx in set ws | ws in Map(f, subsetSeqs(xs[1..])) :: ToSet(ws);
+            // assert forall ss :: ss in PowerSet(ToSet(xs[1..])) ==> ss in seqSeqsToSet(xs[1..]);
+            assert forall ss :: ss in PowerSet(ToSet(xs)) ==> ss in seqSeqsToSet(xs) by {
+                forall ss | ss in PowerSet(ToSet(xs))
+                    ensures ss in seqSeqsToSet(xs)
+                {
+                    if x in ss {
+                        assert ss-{x} in PowerSet(ToSet(xs[1..]));
+                        assert ss-{x} in seqSeqsToSet(xs[1..]);
+                        var yy :| yy in subsetSeqs(xs[1..]) && ToSet(yy) == ss-{x};
+                        assert f(yy) in mapped;
+                        assert ToSet(f(yy)) == ss;
+                        // assert f(ss)
+
+                    }else {
+                        assert ss in PowerSet(ToSet(xs[1..]));
+                    }
+                }
+            }
+
+        }
+    }
+
+    function FindCCliqueNaive<Person(==)>(xs: seq<Person>): seq<seq<Person>>
+        requires distinct(xs)
+    {
+        var people := ToSet(xs);
+        Filter((ss) => IsCelebrityClique(ToSet(ss),  people),subsetSeqs(xs))
+    }
+
+    predicate nonmember<Person(==)>(p: Person, cs: set<Person>) 
+    {
+        forall c :: c in cs ==> Knows(p, c) && !Knows(c, p)
+    }
+
+    lemma mapTest<T,R>(xs: seq<T>, f: T -> R)
+        requires |xs| != 0
+        ensures Map(f, xs)[0] == f(xs[0])
+    {
+
+ 
+        // assert |xs| != 0;
+        // assert |xs| > 0;
+        // assert |xs| == |Map(f, xs)|;
+        // assert xs == [xs[0]]+xs[1..];
+        // var res := Map(f, xs);
+        // assert 0 < |xs|;
+        // assert Map(f, [])  == []; 
+        // assert forall i :: 0 <= i < |xs| ==> res[i] == f(xs[i]);
+        // LemmaMapDistributesOverConcat(f, [xs[0]], xs[1..]);
+        // assert Map(f, [xs[0]]) == [f(xs[0])]+Map(f,[xs[0]][1..]);
+        // assert Map(f, [xs[0]]) == [f(xs[0])]+Map(f,[xs[0]][1..]);
+        // assert res == [f(xs[0])]+Map(f, xs[1..]);
+        // assert res[0] == f(xs[0]);
+    }
+
+    // lemma BirdTransorm<Person>(ps: seq<Person>)
+    //     ensures filter(IsCelebrityClique, subsetSeqs(ps)) ==  filter(nonmember(p), filter(IsCelebrityClique) subsetSeqs)
+    // {
+
+    // }
+
+}
