Pearls/SeqFunctions.dfy
@@ -1,0 +1,104 @@
+
+module SeqFunctions {
+
+    function Map<T,R>(f: (T -> R), xs: seq<T>): (result: seq<R>)
+        ensures |result| == |xs|
+        // ensures forall i {:trigger result[i]} :: 0 <= i < |xs| ==> result[i] == f(xs[i])
+        ensures forall i :: 0 <= i < |xs| ==> result[i] == f(xs[i])
+    {
+        if |xs| == 0 then []
+        else [f(xs[0])] + Map(f, xs[1..])
+    }
+
+    lemma LemmaMapDistributesOverConcat<T,R>(f: (T -> R), xs: seq<T>, ys: seq<T>)
+        ensures Map(f, xs + ys) == Map(f, xs) + Map(f, ys)
+    {
+        reveal Map();
+        if |xs| == 0 {
+        assert xs + ys == ys;
+        } else {
+        calc {
+            Map(f, xs + ys);
+            { assert (xs + ys)[0] == xs[0]; assert (xs + ys)[1..] == xs[1..] + ys; }
+            Map(f, [xs[0]]) + Map(f, xs[1..] + ys);
+            Map(f, [xs[0]]) + Map(f, xs[1..]) + Map(f, ys);
+            {assert [(xs + ys)[0]] + xs[1..] + ys == xs + ys;}
+            Map(f, xs) + Map(f, ys);
+        }
+        }
+    }
+
+function Filter<T>(f: (T -> bool), xs: seq<T>): (result: seq<T>)
+    ensures |result| <= |xs|
+    ensures forall i: nat :: i < |result| ==> f(result[i])
+  {
+    if |xs| == 0 then []
+    else (if f(xs[0]) then [xs[0]] else []) + Filter(f, xs[1..])
+  }
+
+  /* Filtering a sequence is distributive over concatenation. That is, concatenating two sequences 
+     and then using "Filter" is the same as using "Filter" on each sequence separately, and then 
+     concatenating the two resulting sequences. */
+  lemma LemmaFilterDistributesOverConcat<T(!new)>(f: (T -> bool), xs: seq<T>, ys: seq<T>)
+    ensures Filter(f, xs + ys) == Filter(f, xs) + Filter(f, ys)
+  {
+    reveal Filter();
+    if |xs| == 0 {
+      assert xs + ys == ys;
+    } else {
+      calc {
+        Filter(f, xs + ys);
+        { assert {:split_here} (xs + ys)[0] == xs[0]; assert (xs + ys)[1..] == xs[1..] + ys; }
+        Filter(f, [xs[0]]) + Filter(f, xs[1..] + ys);
+        { assert Filter(f, xs[1..] + ys) == Filter(f, xs[1..]) + Filter(f, ys); }
+        Filter(f, [xs[0]]) + (Filter(f, xs[1..]) + Filter(f, ys));
+        { assert {:split_here} [(xs + ys)[0]] + (xs[1..] + ys) == xs + ys; }
+        Filter(f, xs) + Filter(f, ys);
+      }
+    }
+  } 
+
+  function Conj<T>(f: (T -> bool), g: (T -> bool)): (T-> bool) {
+    x => f(x) && g(x)
+  }
+
+  lemma LemmaFilterDistributesOverAnd<T(!new)>(f: (T -> bool), g: (T -> bool), xs: seq<T>)
+    ensures Filter(Conj(f,g), xs) == Filter(f, Filter(g, xs))
+  {
+    if xs == [] {
+
+        assert Filter(Conj(f,g), xs) == Filter(f, Filter(g, xs));
+    } else if |xs| == 1 {
+
+        assert Filter(Conj(f,g), xs) == Filter(f, Filter(g, xs));
+    }else {
+        var x := xs[0];
+        var tail := xs[1..];
+        assert xs == [xs[0]] + xs[1..];
+        LemmaFilterDistributesOverAnd(f,g, xs[1..]);
+        var inner_g_x := Filter(g, [x]);
+        if(f(x) && g(x)) {
+
+            assert Filter(Conj(f,g), xs) == Filter(f, Filter(g, xs));
+        }else{
+            LemmaFilterDistributesOverConcat(Conj(f,g), [xs[0]], xs[1..]);
+            assert Filter(Conj(f,g), [xs[0]]) == [];
+            assert Filter(f, Filter(g, [xs[0]])) == [];
+            assert Filter(f, Filter(g, xs[1..])) == Filter(Conj(f, g), xs[1..]);
+            LemmaFilterDistributesOverConcat(g, [x], tail);
+
+            if !f(x) {
+                LemmaFilterDistributesOverConcat(f, inner_g_x, Filter(g, tail));
+                assert Filter(Conj(f,g), xs) == Filter(f, Filter(g, xs));
+            }else{
+                assert !g(x);
+                assert inner_g_x == [];
+                assert [] + Filter(g, tail) == Filter(g, tail);
+                assert Filter(Conj(f,g), xs) == Filter(f, Filter(g, xs));
+            }
+            assert Filter(Conj(f,g), xs) == Filter(f, Filter(g, xs));
+        }
+        assert Filter(Conj(f,g), xs) == Filter(f, Filter(g, xs));
+    }
+  }
+}
